aarch64 aspec: VCPU+VSpaceRoot objs in Structures
This includes the type-checking fallout from those two main additions,
but no real further validation yet downstream from Structures.thy.

PageTable objects now have an inner object that contains either a
normal page table or a page table with the potentially different size
for top-level VSpace roots.

In ArchVSpaceAcc, the follow-on effects include making pte operations
figure out what kind of object is is by first checking for the
potentially smaller-sized object, and if that does not exist, trying
the larger-sized object (which has a different base address). When
pspace_distinct and pspace_aligned invariants hold, this should model
the behaviour of Haskell/C precisely.

Signed-off-by: Gerwin Klein <gerwin.klein@proofcraft.systems>

spec/abstract/AARCH64/Arch_Structs_A.thy
@@ -1,13 +1,11 @@
 (*
+ * Copyright 2022, Proofcraft Pty Ltd
  * Copyright 2020, Data61, CSIRO (ABN 41 687 119 230)
  *
  * SPDX-License-Identifier: GPL-2.0-only
  *)
 
-(* FIXME AARCH64: verbatim setup copy of RISCV64; needs adjustment and validation;
-                  only minimal type-check changes performed so far if any *)
-
-chapter "RISCV64-Specific Data Types"
+chapter "AARCH64-Specific Data Types"
 
 theory Arch_Structs_A
 imports
@@ -17,7 +15,7 @@ imports
   ExecSpec.Kernel_Config_Lemmas
 begin
 
-context Arch begin global_naming RISCV64_A
+context Arch begin global_naming AARCH64_A
 
 text \<open>
   This theory provides architecture-specific definitions and datatypes including
@@ -27,12 +25,14 @@ text \<open>
 section \<open>Architecture-specific capabilities\<close>
 
 text \<open>
-  The RISCV64 kernel supports capabilities for ASID pools and an ASID controller capability,
+  The AARCH64 kernel supports capabilities for ASID pools and an ASID controller capability,
   along with capabilities for virtual memory mappings.
 \<close>
 
 datatype arch_cap =
-    ASIDPoolCap (acap_obj : obj_ref) (acap_asid_base : asid)
+    ASIDPoolCap
+      (acap_obj : obj_ref)
+      (acap_asid_base : asid)
   | ASIDControlCap
   | FrameCap
       (acap_obj : obj_ref)
@@ -40,18 +40,24 @@ datatype arch_cap =
       (acap_fsize : vmpage_size)
       (acap_is_device : bool)
       (acap_map_data : "(asid \<times> vspace_ref) option")
-  | PageTableCap (acap_obj : obj_ref) (acap_map_data : "(asid \<times> vspace_ref) option")
+  | PageTableCap
+      (acap_obj : obj_ref)
+      (acap_toplevel : bool)
+      (acap_map_data : "(asid \<times> vspace_ref) option")
+  | VCPUCap
+      (acap_obj : obj_ref)
 
 
 text \<open>Update the mapping data saved in a frame or page table capability.\<close>
-definition update_map_data :: "arch_cap \<Rightarrow> (asid \<times> vspace_ref) option \<Rightarrow> arch_cap"
-  where
+definition update_map_data :: "arch_cap \<Rightarrow> (asid \<times> vspace_ref) option \<Rightarrow> arch_cap" where
   "update_map_data cap m \<equiv> case cap of
      FrameCap p R sz dev _  \<Rightarrow> FrameCap p R sz dev m
-   | PageTableCap p _ \<Rightarrow> PageTableCap p m"
+   | PageTableCap p t _ \<Rightarrow> PageTableCap p t m"
 
 
 section \<open>Architecture-specific objects\<close>
+
+subsection \<open>Page tables\<close>
 
 (* This datatype does not match up with the executable spec directly:
    This one here models all "things" one can set on a page or page table entry.
@@ -59,6 +65,7 @@ section \<open>Architecture-specific objects\<close>
 datatype vm_attribute = Global | Execute | User
 type_synonym vm_attributes = "vm_attribute set"
 
+(* FIXME AARCH64: update once C code is there *)
 (* The address of the target object is stored shifted right by pt_bits and stored as a ppn (page
    number). To get the address, use addr_from_pte *)
 type_synonym pte_ppn_len = 52 (* machine_word_len - pt_bits *)
@@ -72,106 +79,151 @@ datatype pte =
   | PagePTE (pte_ppn : pte_ppn) (pte_attr : vm_attributes) (pte_rights : vm_rights)
   | PageTablePTE (pte_ppn : pte_ppn) (pte_attr : vm_attributes)
 
+
+(* who needs dependent types.. *)
+value_type vs_index_len = "if config_ARM_PA_SIZE_BITS_40 then 10 else (9::int)"
+type_synonym vs_index = "vs_index_len word"
+
 type_synonym pt_index_len = 9
 type_synonym pt_index = "pt_index_len word"
 
 text \<open>Sanity check:\<close>
+lemma "LENGTH(vs_index_len) = ptTranslationBits True"
+  by (simp add: ptTranslationBits_def Kernel_Config.config_ARM_PA_SIZE_BITS_40_def)
+
 lemma "LENGTH(pt_index_len) = ptTranslationBits False"
   by (simp add: ptTranslationBits_def)
 
+(* FIXME AARCH64: needs updating for asid map entries and VM ids *)
 type_synonym asid_pool = "asid_low_index \<rightharpoonup> obj_ref"
-type_synonym pt = "pt_index \<Rightarrow> pte"
+
+datatype pt =
+    VSRootPT (the_vs : "vs_index \<Rightarrow> pte")
+  | NormalPT (the_pt : "pt_index \<Rightarrow> pte")
+
+subsection \<open>VCPU\<close>
+
+type_synonym virq = machine_word
+
+end
+
+qualify AARCH64_A (in Arch)
+
+record  gic_vcpu_interface =
+  vgic_hcr  :: word32
+  vgic_vmcr :: word32
+  vgic_apr  :: word32
+  vgic_lr   :: "nat \<Rightarrow> AARCH64_A.virq"
+
+record vcpu =
+  vcpu_tcb  :: "obj_ref option"
+  vcpu_vgic :: "gic_vcpu_interface"
+  vcpu_regs :: "vcpureg \<Rightarrow> machine_word"
+  vcpu_vppi_masked :: "vppievent_irq \<Rightarrow> bool"
+  vcpu_vtimer :: virt_timer
+
+end_qualify
+
+context Arch begin global_naming AARCH64_A
+
+definition "vcpu_sctlr vcpu \<equiv> vcpu_regs vcpu VCPURegSCTLR"
+
+definition default_gic_vcpu_interface :: gic_vcpu_interface where
+  "default_gic_vcpu_interface \<equiv> \<lparr>
+      vgic_hcr  = vgicHCREN,
+      vgic_vmcr = 0,
+      vgic_apr  = 0,
+      vgic_lr   = \<lambda>_. 0
+   \<rparr>"
+
+definition
+  default_vcpu :: vcpu where
+  "default_vcpu \<equiv> \<lparr>
+      vcpu_tcb    = None,
+      vcpu_vgic   = default_gic_vcpu_interface,
+      vcpu_regs   = (\<lambda>_. 0) (VCPURegSCTLR := sctlrDefault),
+      vcpu_vppi_masked = (\<lambda>_. False),
+      vcpu_vtimer = VirtTimer 0
+   \<rparr>"
 
 (* produce discriminators and selectors even though no field names are mentioned *)
 datatype (discs_sels) arch_kernel_obj =
     ASIDPool asid_pool
   | PageTable pt
   | DataPage bool vmpage_size
+  | VCPU vcpu
 
-definition asid_pool_of :: "arch_kernel_obj \<rightharpoonup> asid_pool"
-  where
+definition asid_pool_of :: "arch_kernel_obj \<rightharpoonup> asid_pool" where
   "asid_pool_of ko \<equiv> case ko of ASIDPool pool \<Rightarrow> Some pool | _ \<Rightarrow> None"
 
-definition pt_of :: "arch_kernel_obj \<rightharpoonup> pt"
-  where
+definition pt_of :: "arch_kernel_obj \<rightharpoonup> pt" where
   "pt_of ko \<equiv> case ko of PageTable pt \<Rightarrow> Some pt | _ \<Rightarrow> None"
 
-definition pte_bits :: nat
-  where
+definition vcpu_of :: "arch_kernel_obj \<rightharpoonup> vcpu" where
+  "vcpu_of ko \<equiv> case ko of VCPU vcpu \<Rightarrow> Some vcpu | _ \<Rightarrow> None"
+
+definition pte_bits :: nat where
   "pte_bits = word_size_bits"
 
-definition table_size :: nat
-  where
-  "table_size = ptTranslationBits False + pte_bits"
+definition table_size :: "bool \<Rightarrow> nat" where
+  "table_size is_toplevel = ptTranslationBits is_toplevel + pte_bits"
 
-definition pt_bits :: "nat"
-  where
-  "pt_bits \<equiv> table_size"
+definition pt_bits :: "bool \<Rightarrow> nat" where
+  "pt_bits is_toplevel \<equiv> table_size is_toplevel"
 
-definition addr_from_ppn :: "pte_ppn \<Rightarrow> paddr"
-  where
-  "addr_from_ppn ppn = ucast ppn << pt_bits"
+definition addr_from_ppn :: "pte_ppn \<Rightarrow> paddr" where
+  "addr_from_ppn ppn = ucast ppn << pt_bits False" (* FIXME AARCH64: ppn still unclear *)
 
-abbreviation addr_from_pte :: "pte \<Rightarrow> paddr"
-  where
+abbreviation addr_from_pte :: "pte \<Rightarrow> paddr" where
   "addr_from_pte pte \<equiv> addr_from_ppn (pte_ppn pte)"
 
-primrec arch_obj_size :: "arch_cap \<Rightarrow> nat"
-  where
+primrec arch_obj_size :: "arch_cap \<Rightarrow> nat" where
   "arch_obj_size (ASIDPoolCap _ _) = pageBits"
 | "arch_obj_size ASIDControlCap = 0"
 | "arch_obj_size (FrameCap _ _ sz _ _) = pageBitsForSize sz"
-| "arch_obj_size (PageTableCap _ _ ) = table_size"
+| "arch_obj_size (PageTableCap _ is_toplevel _ ) = table_size is_toplevel"
+| "arch_obj_size (VCPUCap _) = pageBits" (* FIXME AARCH64: vcpuBits not in scope *)
 
-fun arch_cap_is_device :: "arch_cap \<Rightarrow> bool"
-  where
+fun arch_cap_is_device :: "arch_cap \<Rightarrow> bool" where
   "arch_cap_is_device (FrameCap _ _ _ is_dev _) = is_dev"
 | "arch_cap_is_device _ = False"
 
-definition cte_level_bits :: nat
-  where
+definition cte_level_bits :: nat where
   "cte_level_bits \<equiv> 5"
 
-definition tcb_bits :: nat
-  where
+definition tcb_bits :: nat where
   "tcb_bits \<equiv> 10"
 
-definition endpoint_bits :: nat
-  where
+definition endpoint_bits :: nat where
   "endpoint_bits \<equiv> 4"
 
-definition ntfn_bits :: nat
-  where
+definition ntfn_bits :: nat where
   "ntfn_bits \<equiv> 5"
 
-definition untyped_min_bits :: nat
-  where
+definition untyped_min_bits :: nat where
   "untyped_min_bits \<equiv> 4"
 
-definition untyped_max_bits :: nat
-  where
-  "untyped_max_bits \<equiv> 38"
+definition untyped_max_bits :: nat where
+  "untyped_max_bits \<equiv> 47"
 
-primrec arch_kobj_size :: "arch_kernel_obj \<Rightarrow> nat"
-  where
+primrec arch_kobj_size :: "arch_kernel_obj \<Rightarrow> nat" where
   "arch_kobj_size (ASIDPool _) = pageBits"
-| "arch_kobj_size (PageTable _) = table_size"
+| "arch_kobj_size (PageTable pt) = table_size (is_VSRootPT pt)"
 | "arch_kobj_size (DataPage _ sz) = pageBitsForSize sz"
+| "arch_kobj_size (VCPU _) = pageBits" (* FIXME AARCH64: vcpuBits not in scope *)
 
-fun aobj_ref :: "arch_cap \<rightharpoonup> obj_ref"
-  where
+fun aobj_ref :: "arch_cap \<rightharpoonup> obj_ref" where
   "aobj_ref ASIDControlCap = None"
 | "aobj_ref c = Some (acap_obj c)"
 
-definition acap_rights_update :: "cap_rights \<Rightarrow> arch_cap \<Rightarrow> arch_cap"
-  where
+definition acap_rights_update :: "cap_rights \<Rightarrow> arch_cap \<Rightarrow> arch_cap" where
   "acap_rights_update R acap \<equiv>
     case acap of
       FrameCap ref cR sz dev as \<Rightarrow> FrameCap ref (validate_vm_rights R) sz dev as
     | _ \<Rightarrow> acap"
 
 text \<open>Sanity check:\<close>
-lemma "LENGTH(pte_ppn_len) = word_bits - pt_bits"
+lemma "LENGTH(pte_ppn_len) = word_bits - pt_bits False"
   by (simp add: pte_bits_def ptTranslationBits_def word_size_bits_def word_bits_def
                 pt_bits_def table_size_def)
 
@@ -182,123 +234,117 @@ datatype aobject_type =
   | LargePageObj
   | HugePageObj
   | PageTableObj
-  | ASIDPoolObj
+  | VSpaceRootObj
+  | ASIDPoolObj (* used internally, not on API level *)
+  | VCPUObj
 
-definition arch_is_frame_type :: "aobject_type \<Rightarrow> bool"
-  where
+definition arch_is_frame_type :: "aobject_type \<Rightarrow> bool" where
   "arch_is_frame_type aobj \<equiv> aobj \<noteq> PageTableObj"
 
-definition arch_default_cap :: "aobject_type \<Rightarrow> obj_ref \<Rightarrow> nat \<Rightarrow> bool \<Rightarrow> arch_cap"
-  where
+definition arch_default_cap :: "aobject_type \<Rightarrow> obj_ref \<Rightarrow> nat \<Rightarrow> bool \<Rightarrow> arch_cap" where
   "arch_default_cap tp r n dev \<equiv> case tp of
-     SmallPageObj \<Rightarrow> FrameCap r vm_read_write ARMSmallPage dev None
-   | LargePageObj \<Rightarrow> FrameCap r vm_read_write ARMLargePage dev None
-   | HugePageObj  \<Rightarrow> FrameCap r vm_read_write ARMHugePage dev None
-   | PageTableObj \<Rightarrow> PageTableCap r None
-   | ASIDPoolObj  \<Rightarrow> ASIDPoolCap r 0" (* unused, but nicer properties when defined *)
+     SmallPageObj  \<Rightarrow> FrameCap r vm_read_write ARMSmallPage dev None
+   | LargePageObj  \<Rightarrow> FrameCap r vm_read_write ARMLargePage dev None
+   | HugePageObj   \<Rightarrow> FrameCap r vm_read_write ARMHugePage dev None
+   | PageTableObj  \<Rightarrow> PageTableCap r False None
+   | VSpaceRootObj \<Rightarrow> PageTableCap r True None
+   | VCPUObj       \<Rightarrow> VCPUCap r
+   | ASIDPoolObj   \<Rightarrow> ASIDPoolCap r 0" (* unused, but nicer properties when defined *)
 
-definition default_arch_object :: "aobject_type \<Rightarrow> bool \<Rightarrow> nat \<Rightarrow> arch_kernel_obj"
-  where
+definition default_arch_object :: "aobject_type \<Rightarrow> bool \<Rightarrow> nat \<Rightarrow> arch_kernel_obj" where
   "default_arch_object tp dev n \<equiv> case tp of
-     SmallPageObj \<Rightarrow> DataPage dev ARMSmallPage
-   | LargePageObj \<Rightarrow> DataPage dev ARMLargePage
-   | HugePageObj  \<Rightarrow> DataPage dev ARMHugePage
-   | PageTableObj \<Rightarrow> PageTable (\<lambda>_. InvalidPTE)
-   | ASIDPoolObj  \<Rightarrow> ASIDPool Map.empty"
+     SmallPageObj  \<Rightarrow> DataPage dev ARMSmallPage
+   | LargePageObj  \<Rightarrow> DataPage dev ARMLargePage
+   | HugePageObj   \<Rightarrow> DataPage dev ARMHugePage
+   | PageTableObj  \<Rightarrow> PageTable (NormalPT (\<lambda>_. InvalidPTE))
+   | VSpaceRootObj \<Rightarrow> PageTable (VSRootPT (\<lambda>_. InvalidPTE))
+   | ASIDPoolObj   \<Rightarrow> ASIDPool Map.empty"
 
-(* FIMXE AARCH64: needs to be defined in design/AARCH64/Arch_Structs_B.thy  *)
-(*
 type_synonym arm_vspace_region_uses = "vspace_ref \<Rightarrow> arm_vspace_region_use"
-*)
 
 text \<open>
   The number of levels over all virtual memory tables.
-  For RISC-V, we have three page table levels plus the ASID pool level.
+  For AARCH64 in hyp without @{const config_ARM_PA_SIZE_BITS_40}, we have four page table
+  levels plus the ASID pool level.
 
   The top level (with the highest number) contains ASID pools, the next levels contain the
   top-level page tables, and level 1 page tables. The bottom-level page tables (level 0)
   contains only InvalidPTEs or PagePTEs.
 \<close>
-type_synonym vm_level = 4
+(* FIXME AARCH64: this depends on config_ARM_PA_SIZE_BITS_40 *)
+type_synonym vm_level = 5
 
-definition asid_pool_level :: vm_level
-  where
+definition asid_pool_level :: vm_level where
   "asid_pool_level = maxBound"
 
-definition max_pt_level :: vm_level
-  where
+definition max_pt_level :: vm_level where
   "max_pt_level = asid_pool_level - 1"
 
 end
 
-qualify RISCV64_A (in Arch)
+qualify AARCH64_A (in Arch)
 
 section \<open>Architecture-specific state\<close>
 
 record arch_state =
-  riscv_asid_table :: "asid_high_index \<rightharpoonup> obj_ref"
-  riscv_global_pts :: "RISCV64_A.vm_level \<Rightarrow> obj_ref set"
-(* FIXME AARCH64: add when type def above works
-  riscv_kernel_vspace :: "obj_ref \<Rightarrow> RISCV64_H.riscvvspace_region_use" *)
+  arm_asid_table :: "asid_high_index \<rightharpoonup> obj_ref"
+  (* FIXME AARCH64: add arm_hwasid_table *)
+  (* FIXME AARCH64: add arm_next_asid *)
+  arm_us_global_vspace :: "obj_ref"
+  arm_kernel_vspace :: "AARCH64_A.arm_vspace_region_uses"
+  arm_current_vcpu    :: "(obj_ref \<times> bool) option"
+  arm_gicvcpu_numlistregs :: nat
 
-text \<open>
-  The @{const riscv_global_pts} generalise the concept of global page tables.
-  The invariants will constrain the set of tables for @{term max_pt_level} to a
-  singleton, and for @{term asid_pool_level} to empty. All other levels may contain
-  multiple or no tables, depending on how kernel initialisation sets up the kernel window.
-\<close>
 
 end_qualify
 
-context Arch begin global_naming RISCV64_A
+context Arch begin global_naming AARCH64_A
 
 section "Type declarations for invariant definitions"
 
 datatype aa_type =
     AASIDPool
-  | APageTable
+  | APageTable bool (* is_toplevel *)
+  | AVCPU
   | AUserData vmpage_size
   | ADeviceData vmpage_size
 
-definition aa_type :: "arch_kernel_obj \<Rightarrow> aa_type"
-  where
+definition aa_type :: "arch_kernel_obj \<Rightarrow> aa_type" where
   "aa_type ao \<equiv> case ao of
-     PageTable pt    \<Rightarrow> APageTable
+     PageTable pt    \<Rightarrow> APageTable (is_VSRootPT pt)
    | DataPage dev sz \<Rightarrow> if dev then ADeviceData sz else AUserData sz
-   | ASIDPool f      \<Rightarrow> AASIDPool"
+   | ASIDPool _      \<Rightarrow> AASIDPool
+   | VCPU _          \<Rightarrow> AVCPU"
 
-definition badge_bits :: nat
-  where
+definition badge_bits :: nat where
   "badge_bits \<equiv> 64"
 
 end
 
 section "Arch-specific TCB"
 
-qualify RISCV64_A (in Arch)
+qualify AARCH64_A (in Arch)
 
 text \<open> Arch-specific part of a TCB: this must have at least a field for user context. \<close>
 record arch_tcb =
   tcb_context :: user_context
+  tcb_vcpu    :: "obj_ref option"
 
 end_qualify
 
-context Arch begin global_naming RISCV64_A
+context Arch begin global_naming AARCH64_A
 
-definition default_arch_tcb :: arch_tcb
-  where
-  "default_arch_tcb \<equiv> \<lparr>tcb_context = new_context\<rparr>"
+definition default_arch_tcb :: arch_tcb where
+  "default_arch_tcb \<equiv> \<lparr>tcb_context = new_context, tcb_vcpu = None\<rparr>"
 
 text \<open>
   Accessors for @{text "tcb_context"} inside @{text "arch_tcb"}. These are later used to
   implement @{text as_user}, i.e.\ need to be compatible with @{text user_monad}.
 \<close>
-definition arch_tcb_context_set :: "user_context \<Rightarrow> arch_tcb \<Rightarrow> arch_tcb"
-  where
+definition arch_tcb_context_set :: "user_context \<Rightarrow> arch_tcb \<Rightarrow> arch_tcb" where
   "arch_tcb_context_set uc a_tcb \<equiv> a_tcb \<lparr> tcb_context := uc \<rparr>"
 
-definition arch_tcb_context_get :: "arch_tcb \<Rightarrow> user_context"
-  where
+definition arch_tcb_context_get :: "arch_tcb \<Rightarrow> user_context" where
   "arch_tcb_context_get a_tcb \<equiv> tcb_context a_tcb"
 
 text \<open>
